\documentclass[danish,english,10pt,a4paper]{article}
\input{../Preamble}

\title{Workshop 1, Week 2, Friday}
\begin{document}
\maketitle

\section*{1}
Prove: $\forall n \in \mathbb{Z}$, if \textit{n} is even, then $n^2$ is even.
\\
\\
If $n= 2x$ n is even. Insert \textit{n} will give $n^2 = (2x)^2 \Leftrightarrow n^2=4x^2=2(2x^2)$ which is the even since 2 times an integer is even.


\section*{2}
Prove: $\forall n_1, n_2 \in \mathbb{Z}$, if $n_1$ and $n_2$ is even, then $n_1+n_2$ is even.
\\
\\
Same as above: insert $x^2$ in $n_1$ and $n_2$ which gives even integer, since an even integer added with an even integer equals an even integer. $2k_1 + 2k_2 \Leftrightarrow 2(k_1+k_2)$


\section*{3}


\section*{4}
Prove: Let $x \in \mathbb{Z}$ If $7x+5$ is odd, then \textit{x} is even.
\\
\\
Assume \textit{x} is odd. Then $x=2y+1$ (definition) where $y \in \mathbb{Z}$.\\
$7x+5 = 7(2y+1)+5 = 14y+7+5 = 14y+12 = 2(7y+6)$. 
\\
Since $7y+6$ is an integer, $7x+5$ is even.


\section*{5}
Let $n \in \mathbb{N}$. Then \textit{n} is even if and only if $3n^2+8$ is even.
\begin{align*}
3n^2+8 &= 3(2x)^2+8\\
	&= 3\cdot 4x^2+8\\
	&= 12x^2+8 \\
	&= 2(6x^2+4) & \text{even natural + even natural = even natural}	
\end{align*}
Same with a \textbf{contriduction} -- If \textit{n} is odd then the second statement is odd.
\begin{align*}
3n^2+8 &= 3(2x+1)^2+8 & 2x+1 \text{ is odd}\\
	&=3(2x^2+1+2x)+8\\
	&=6x^2+3+6x+8\\
	&=2(3x^2+3x+5)+1 & \text{proven odd}
\end{align*}


\section*{6}
Let $n \in \mathbb{Z}$. Then $n^2-3n+9$ is odd:
\\
Case 1:
\begin{align*}
n^2-3n+9 &= (2x)^2-3(2x)+9 & n \text{ is even}\\
	&=4x^2-6x+9	\\
	&=2(2x^2-3x+4)+1 & \text{equals odd}
\end{align*}
Case 2:
\begin{align*}
n^2-3n+9 &= (2x+1)^2-3(2x+1)+9 & n \text{ is odd}\\
	&=4x^2+1+2x-6x-3+9	\\
	&=2(2x^2-2x+3)+1 & \text{equals odd}
\end{align*}
Since the P = odd integers and Q = even integers, then $\mathbb{Z} = P \cup Q$.


\end{document}